@prefix dcterms: <http://purl.org/dc/terms/>.
@prefix foaf: <http://xmlns.com/foaf/0.1/>.
@prefix owl: <http://www.w3.org/2002/07/owl#>.
@prefix xsd: <http://www.w3.org/2001/XMLSchema#>.
@prefix xml: <http://www.w3.org/XML/1998/namespace>.
@prefix voaf: <http://purl.org/vocommons/voaf#>.
@prefix rdfs: <http://www.w3.org/2000/01/rdf-schema#>.
@prefix rdf: <http://www.w3.org/1999/02/22-rdf-syntax-ns#>.
@prefix wdrs: <http://www.w3.org/2007/05/powder-s#>.
@prefix schema: <http://schema.org/> .
@prefix cc: <http://creativecommons.org/ns#>.
@prefix vann: <http://purl.org/vocab/vann/>.
@prefix skos: <http://www.w3.org/2004/02/skos/core#>.
@prefix : <http://www.w3.org/ns/person#>.

<http://www.w3.org/ns/person> a voaf:Vocabulary, owl:Ontology;
	dcterms:title "ISA Programme Person Core Vocabulary"@en;
	dcterms:comment """This vocabulary was not developed by a W3C group and its publication does not imply endorsement
		by the W3C Membership. Terms MAY be deprecated or their definitions clarified but they will
		not be deleted (see the W3C Persistence Policy). The vocabulary MAY be further developed by a future group.""";
	dcterms:abstract "The Person Core Vocabulary provides a minimum set of classes and properties for describing a natural person, i.e. the individual as opposed to any role they may play in society or the relationships they have to other people, organisations and property; all of which contribute significantly to the broader concept of identity."@en;
	dcterms:creator [schema:affiliation <http://www.w3.org/data#W3C>;
		rdfs:seeAlso <http://philarcher.org/foaf.rdf#me>;
		foaf:homepage <http://www.w3.org/People/all#phila>;
		foaf:name "Phil Archer"] ,
		[schema:affiliation [foaf:homepage <http://ies.jrc.ec.europa.eu/DE>;
		foaf:name "European Commission, Joint Research Centre "];
		rdfs:seeAlso <http://andrea-perego.name/foaf/#me>;
		foaf:homepage <http://andrea-perego.name/>;
		foaf:name "Andrea Perego"];
	foaf:maker[foaf:name "Core Vocabularies Working Group (Person Task Force)";
	foaf:page <http://joinup.ec.europa.eu/asset/core_person/home>];
	dcterms:description "The Person Core Vocabulary provides a minimum set of classes and properties for describing a natural person, i.e. the individual as opposed to any role they may play in society or the relationships they have to other people, organisations and property; all of which contribute significantly to the broader concept of identity.";
	dcterms:issued "2012-05-07"^^xsd:date;
	dcterms:modified "2013-11-17"^^xsd:date;
	dcterms:modified "2013-12-21"^^xsd:date; # Corrected schema URI to http://www.w3.org/ns/person (no #)
	vann:preferredNamespacePrefix "person";
	vann:preferredNamespaceUri "http://www.w3.org/ns/person#";
	wdrs:describedby <https://joinup.ec.europa.eu/asset/core_person/asset_release/core-person-vocabulary-100>;
	dcterms:license <https://joinup.ec.europa.eu/category/licence/isa-open-metadata-licence-v11>;
	dcterms:rights "Copyright &#169; 2012 European Commission".

<https://joinup.ec.europa.eu/category/licence/isa-open-metadata-licence-v11>
	dcterms:title "ISA Open Metadata Licence v1.1";
	cc:attributionName "European Commission";
	cc:attributionURL <http://ec.europa.eu/>.

:Person dcterms:identifier "person:Person";
	a rdfs:Class;
	rdfs:label "Person"@en;
	rdfs:comment "An individual person who may be dead or alive, but not imaginary. It is that restriction that makes person:Person a sub class of both foaf:Person and schema:Person which both cover imaginary characters as well as real people."@en;
	rdfs:isDefinedBy <http://www.w3.org/ns/person>;
	rdfs:subClassOf foaf:Person;
	rdfs:subClassOf schema:Person.

:patronymicName dcterms:identifier "person:patronymicName";
	a rdf:Property, owl:DatatypeProperty;
	rdfs:label "patronymic name"@en;
	rdfs:comment "Patronymic names refer to a father's given name, not the family name inherited from the mother and father as is the case in countries such as Spain and Portugal."@en;
	vann:usageNote "Patronymic names are important in some countries. Iceland does not have a concept of family name in the way that many other European countries do, for example. In Bulgaria and Russia, patronymic names are in every day usage, for example, the &quot;Sergeyevich&quot; (Ð¡ÐµÑ€Ð³ÐµÐµÐ²Ð¸Ñ‡) in &quot;Mikhail Sergeyevich Gorbachev&quot; (ÐœÐ¸Ñ…Ð°Ð¸Ð» Ð¡ÐµÑ€Ð³ÐµÐµÐ²Ð¸Ñ‡ Ð“Ð¾Ñ€Ð±Ð°Ñ‡Ñ‘Ð²)."@en;
	rdfs:domain :Person;
	rdfs:range rdfs:Literal;
	rdfs:isDefinedBy <http://www.w3.org/ns/person>.

:birthName dcterms:identifier "person:birthName";
	a rdf:Property, owl:DatatypeProperty;
	rdfs:label "birth name"@en;
	rdfs:comment "TODO"@en;
	vann:usageNote "All data associated with an individual is subject to change. Names can change for a variety of reasons, either formally or informally, and new information may come to light that means that a correction or clarification can be made to an existing record. Birth names tend to be persistent however and for this reason they are recorded by some public sector information systems. There is no granularity for birth name - the full name should be recorded in a single field."@en;
	rdfs:domain :Person;
	rdfs:range rdfs:Literal;
	rdfs:isDefinedBy <http://www.w3.org/ns/person>.

:placeOfBirth dcterms:identifier "person:placeOfBirth";
	a rdf:Property, owl:ObjectProperty;
	rdfs:comment "A person's place of birth."@en;
	rdfs:isDefinedBy <http://www.w3.org/ns/person>;
	rdfs:label "place of birth"@en;
	rdfs:domain :Person;
	rdfs:range dcterms:Location;
	rdfs:range schema:Place.

:placeOfDeath dcterms:identifier "person:placeOfDeath";
	a rdf:Property, owl:ObjectProperty;
	rdfs:comment "A person's place of death."@en;
	rdfs:isDefinedBy <http://www.w3.org/ns/person>;
	rdfs:label "place of death"@en;
	rdfs:domain :Person;
	rdfs:range dcterms:Location;
	rdfs:range schema:Place.

:countryOfBirth dcterms:identifier "person:countryOfBirth";
	a rdf:Property,	owl:ObjectProperty;
	rdfs:comment "The country in which a Person was born."@en;
	rdfs:isDefinedBy <http://www.w3.org/ns/person>;
	rdfs:label "country of birth"@en;
	rdfs:domain :Person;
	rdfs:range dcterms:Location;
	rdfs:range schema:Place.

:countryOfDeath dcterms:identifier "person:countryOfDeath";
	a rdf:Property,	owl:ObjectProperty;
	rdfs:comment "The country in which a Person died."@en;
	rdfs:isDefinedBy <http://www.w3.org/ns/person>;
	rdfs:label "country of death"@en;
	rdfs:domain :Person;
	rdfs:range dcterms:Location;
	rdfs:range schema:Place.

:citizenship dcterms:identifier "person:citizenship";
	a rdf:Property,	owl:ObjectProperty;
	rdfs:comment "The citizenship relationship links a Person to a Jurisdiction that has conferred citizenship rights on the individual such as the right to vote, to receive certain protection from the community or the issuance of a passport. Multiple citizenships are recorded as multiple instances of the citizenship relationship."@en;
	rdfs:isDefinedBy <http://www.w3.org/ns/person>;
	rdfs:label "citizenship"@en;
	skos:altLabel "nationality"@en; # See spec: Citizenship is information needed by many cross-border use cases and is a legal status as opposed to the more culturally-focussed and less well-defined term "nationality." 
	rdfs:domain :Person;
	rdfs:range dcterms:Jurisdiction.

:residency dcterms:identifier "person:residency";
	a rdf:Property,	owl:ObjectProperty;
	rdfs:comment "Residency typically provides an individual with a subset of the rights of a citizen."@en;
	rdfs:isDefinedBy <http://www.w3.org/ns/person>;
	rdfs:label "residency"@en;
	rdfs:domain :Person;
	rdfs:range dcterms:Jurisdiction.

foaf:name a rdf:Property;
	rdfs:label "full name"@en;
	rdfs:comment "The full name contains the complete name of a person  as one string. In addition to the content of given name, family name and, in some systems, patronymic name, this can carry additional parts of a person's name such as titles, middle names or suffixes like "the third" or names which are neither a given nor a family name."@en;
	vann:usageNote "The Full Name is the most reliable label for an individual and as such its use is strongly encouraged, irrespective of whether that name is broken down using the more granular elements. It is anticipated that some systems will only provide or process the full name of a person. Where an individual has more than one full legal name (a relatively rare but not unknown phenomenon), the full name property can be used more than once. In this case, however, the granular name elements should not be used since the intention is that these provide a breakdown of the full name and it will not be clear of which full name this is true."@en;
	vann:usageNote "A name usually sticks with a person for a long time period. In some European countries a name may only be changed according to certain laws and life events, e.g. marriage. The name denominates a natural person even if he/she changes their address. Documents like birth certificate or diploma usually don’t carry an address but always the name. Thus the name is one of the core attributes. However it is not sufficient to identify a person since there are combinations of very common names like Smith in the UK, Meier in Germany, or Li in China."@en;
	rdfs:range rdfs:Literal.
	
foaf:familyName a rdf:Property;
	rdfs:label "family name"@en;
	skos:altLabel "surname"@en;
	rdfs:comment "A family name is usually shared by members of a family."@en;
	vann:usageNote "This attribute also carries prefixes or suffixes which are part of the Family Name, e.g. “de Boer”, “van de Putte”, “von und zu Orlow”. Multiple family names, such as are commonly found in Hispanic countries, are recorded in the single Family Name field so that, for example, Miguel de Cervantes Saavedra's Family Name would be recorded as "de Cervantes Saavedra"."@en;
	rdfs:range rdfs:Literal.
	
foaf:givenName a rdf:Property;
	rdfs:label "given name"@en;
	skos:altLabel "forename"@en;
	rdfs:comment "A given name, or multiple given names, are the denominator(s) that identify an individual within a family."@en;
	vann:usageNote "These are given to a person by his or her parents at birth or may be legally recognised as 'given names' through a formal process. All given names are ordered in one field so that, for example, the Given Name for Johann Sebastian Bach is 'Johann Sebastian.'"@en;
	rdfs:range rdfs:Literal.
	
dcterms:alternative a rdf:Property;
	rdfs:label "alternative name"@en;
	rdfs:comment "Any name by which an individual is known other than their full name.";
	vann:usageNote "Many individuals use a short form of their name, a 'middle' name as a 'first' name or a professional name. For example, the British politician and former UN High Representative for Bosnia and Herzegovina, Jeremy John Durham Ashdown, Baron Ashdown of Norton-sub-Hamdon, is usually referred to simply as 'Paddy Ashdown' or 'Lord Ashdown.'"@en;
	vann:usageNote "It is not the role of the alternative name property to record nick names, pet names or other 'familiar names' that will be of no consequence in public sector data exchange. Furthermore, some individuals have more than one legal name in which case the full name property should be used multiple times. Alternative name gives a means of recording names by which an individual is generally known, or professionally known, even though such names are no more than secondary from a legal point of view. "@en;
	rdfs:range rdfs:Literal.
	
schema:birthDate a rdf:Property;
	rdfs:label "date of birth";
	rdfs:comment "A date that specifies the birth date of a person.";
	rdfs:range xsd:DateTime;
	
schema:deathDate a rdf:Property;
	rdfs:label "date of death";
	rdfs:comment "A date that specifies the death date of a person.";
	rdfs:range xsd:DateTime;
	
schema:gender a rdf:Property;
	rdfs:label "gender"@en;
	rdfs:comment "The gender of an individual should be recorded using a controlled vocabulary that is appropriate for the specific context. In some cases the chromosomal or physical state of an individual will be more important than the gender that they express, in others the reverse will be true. What is always important is that the controlled vocabulary used to describe an individual's gender is stated explicitly."@en;
	rdfs:range skos:Concept.
	
	